\documentclass{school-22.101-notes}
\date{October 12, 2011}

\begin{document}
\maketitle

%%%%%%%%%%%%%%%%%%%%%%%%%%% Angular Momentum %%%%%%%%%%%%%%%%%%%%
\lecture{Angular Momentum}
Angular momentum is a conserved quantity in a central force field. While a general potential is dependent on the spatial coordinate:
\eqn{ V(\uline{x}) = V(r,\theta, \phi)   }
a special potential that is only depend on radius (no $\theta, \phi$ dependency) is called a central force field because of its rotational symmetry. 


%%%%%%%%%%%%%%% 12 Fall %%%%%%%%%%%%%%%%%
\topic{Physical Meaning of Momentums}
\textbf{Momentum is a generator of translation.}\footnote{This lecture is given on Oct. 1, 2012 by Prof. Ju Li.} We consider an operator $T$ that moves a $\psi(x)$ to $\psi(x-\Delta x)$: 
\eqn{ T \psi(x) = \psi(x-\Delta x)} 
We perform the Taylor expansion on $\psi(x - \Delta x)$: 
\begin{align}
  \psi(x - \Delta x) &= \psi(x) + (-\Delta x) \ppsipx + \frac{(-\Delta x)^2}{2!} \ppsipxn2 + \frac{(-\Delta x)^3}{3!} \ppsipxn3 + \cdots \\
  &= \left[ 1 - \Delta x \ppx + \frac{(-\Delta x \ppxn2)^2}{2!} + \frac{(-\Delta x \ppxn3)^3}{3!} + \cdots \right] \psi(x) 
\end{align}
Using $e^x = 1 + x + \frac{x^2}{2!} + \frac{x^3}{3!} + \cdots$, we can write, 
\begin{align}
  \psi(x - \Delta x) &= \exp \left( -\Delta x \ppx \right) \psi(x) \\
  &= \exp \left(- \frac{i \Delta x (-i \hbar \ppx)}{\hbar} \right) \psi(x) \\
  &= \exp \left(-\frac{i \Delta x \cdot \hat{P} }{\hbar} \right) \psi(x) \label{momentum-meaning}
\end{align}

Eq.~\ref{momentum-meaning} implies that the position transform vector is the momentum operator. 


\textbf{Angular momentum is a generator of rotation.} We consider an operator $R(n, \theta)$ that rotate a $\psi$ to $\psi_{\mathrm{rot}}$: 
\eqn{ R(\vec{n}, \theta) \psi = \psi_{\mathrm{rot}} }
We can prove that 
\eqn{ R(\vec{n}, \theta) = \exp \left( - \frac{i \theta}{\hbar} \vec{n} \cdot \vec{J} \right) \label{scalar-R} }
where $\vec{n}$ is the axis of rotation, $\theta$ is the amount of rotation in radian.  Keep in mind this $R(\vec{n}, \theta)$ is a scalar operator. 


\topic{A Mathematical Approach: How Angular Momentum Commutes With Others}
Now we are going to approach a measurement of an arbitrary vector operator $V$(the vector notation is ommited in this section) from two angles:
\begin{enumerate}
\item Recall the expression for $R(\vecn, \theta)$ in Eq.~\ref{scalar-R}. Then for an arbitrary vector operator $V$, a measurement can be written as, 
\eqn{ \bra{\psi} R^+ V R \ket{\psi} &= \bra{\psi} \exp \left( \frac{i \theta \vec{n} \cdot \vec{J} }{\hbar} \right) V \exp \left( - \frac{i \theta \vec{n} \cdot \vec{J} }{\hbar} \right) \ket{\psi}   \label{mom-phy-ang} }
For small $\theta$, we can Taylor expand the RHS of Eq.~\ref{mom-phy-ang}, 
\eqn{ \exp \left( \frac{i \theta \vec{n} \cdot \vec{J} }{\hbar} \right) V \exp \left( - \frac{i \theta \vec{n} \cdot \vec{J} }{\hbar} \right) = V + \frac{i \theta}{\hbar} [\vec{n} \cdot \vec{j}, V] + O(\theta^2) }
That is, the measurement becomes, 
\eqn{ \bra{\psi} V + \frac{i \theta}{\hbar} [\vec{n} \cdot \vec{j}, V] \ket{\psi}  \label{measurement-1} }

\item If we prepare a $\psi_{\mathrm{rot}}$, measure the expectation of $V$, the result should be a rotated version of expectation of the original measurement. That is, there is a 3x3 rotation matrix (matrix of numbers, not operators) with the following property: 
\eqn{ \bra{\psi_{\mathrm{rot}}} V \ket{\psi_{\mathrm{rot}}} &= \vec{R}(\vec{n}, \theta) \bra{\psi} V \ket{\psi}  }
Again we Taylor expand for small $\theta$, 
\eqn{ \vec{R} (\vecn, \theta) V = V + \theta (\vec{n} \cross V ) + O (\theta^2) }
The the measurement becomes, 
\eqn{ \bra{\psi} V + \theta (\vec{n} \cross V ) \ket{\psi}  \label{measurement-2}  }
\end{enumerate}
The two ways should yield same result, so we can equate Eq.~\ref{measurement-1} and Eq.~\ref{measurement-2}: 
\begin{align}
\bra{\psi} V + \frac{i \theta}{\hbar} [\vec{n} \cdot \vec{j}, V] \ket{\psi}  &=  \bra{\psi} V + \theta (\vec{n} \cross V ) \ket{\psi} \\
\bra{\psi}  \frac{i \theta}{\hbar} [\vec{n} \cdot \vec{j}, V] \ket{\psi}  &=  \bra{\psi} \theta (\vec{n} \cross V ) \ket{\psi} \\
\bra{\psi}  \frac{i}{\hbar} [\vec{n} \cdot \vec{j}, V] \ket{\psi}  &=  \bra{\psi} \vec{n} \cross V \ket{\psi} \\
\bra{\psi} \frac{i}{\hbar} [n_j J_j, V] \ket{\psi}  &= \vec{n} \cross \bra{\psi} V \ket{\psi} \\
\bra{\psi} \frac{i}{\hbar} [n_j J_j, V_i] \ket{\psi} &= \epsilon_{i,j,k} n_j \bra{\psi} V_k \ket{\psi} \\
\frac{i}{\hbar} [J_j, V_i] &= \epsilon_{ijk} V_k \\
\Aboxed{ [V_i, J_j] &= i \hbar \epsilon_{ijk} V_k }  \label{J-basic}
\end{align}

Recall that $[\vec{x}, \vec{P} ] = i \hbar \epsilon_{ijk} V_k$. Thus, 
\eqn{ \Aboxed{ \vec{J} &= \vec{L} = \vec{x} \cross \vec{P}  } \label{defn-J} }

\clearpage
Now that we know some fundamental properties of $\vec{J}$, we can do the following to make use of them.
\begin{enumerate}
\item We define a $J^2$ term,
  \eqn{ J^2 &= \vec{J} \cdot \vec{J} = J_x^2 + J_y^2 + J_z^2 = J_i J_i }
  Using $[AB,C] = A[B,C] + [A,C] B$, 
  \eqn{ [J^2, J_3] &= [J_i J_i, J_3] = J_i [J_i, J_3] + [J_i, J_3] J_i }
  Apply Eq.~\ref{J-basic} on the $[J_i, J_3]$ terms,
  \eqn{ [J^2,J_3] &= J_i (i \hbar \epsilon_{i3k} J_k) + (i\hbar \epsilon_{i3k} J_k) J_i  = i\hbar \epsilon_{i3k} (J_i J_k + J_k J_i) = 0 }
  Basically \hi{$J^2$ commutes with any projection of $J$}, 
  \eqn{ \boxed{ [J^2, \vecn \cdot \vec{J} ] = [J^2, n_x J_x + n_y J_y + n_z J_z] = 0}  }
  which includes, 
  \eqn{ [J^2, J_x] &= 0,  & [J^2, J_y] &=0, &[J^2, J_z]&=0, & [J^2,J_+]&=0, & [J^2, J_-]&= 0 }

\item We define the raising operator $J_+ = J_x + iJ_y$, and the lowering operator $J_- = J_x - iJ_y$. As we've seen above, $[J^2, J_+] = [J^2, J_-] = 0$. Next we show how $J_+, J_-$ relate to $J_z$: 
  \begin{enumerate}
  \item To start we plug in the definition and use Eq.~\ref{J-basic}, 
    \eqn{ [J_z, J_+] = [J_z, J_x + i J_y] = i \hbar J_y + i (-i \hbar J_x) = \hbar J_+   } 
    \eqn{ [J_z, J_-] = [J_z, J_x - i J_y]  = (i \epsilon_{231} J_x - \epsilon_{132} J_y) i \hbar = - \hbar (J_x - i J_y)  = -\hbar J_- }


  \item We add an arbitrary basis $\ket{z}$ to both side (called simultaneously diagonalize $J^2$ and $J_z$),  
    \eqn{ [J_z, J_-] \ket{z} &= - \hbar J_- \ket{z} \label{Eq1} }
    We define, 
    \eqn{ J_z \ket{z} = z \hbar \ket{z} \label{eigen-Jz} }
    Then we can simplify the LHS of Eq.~\ref{Eq1}: 
    \eqn{ [J_z, J_-] \ket{z}  = J_z J_- \ket{z} - J_- J_z \ket{z} = J_z J_- \ket{z} -  J_- z \hbar \ket{z} \label{Eq2} }
    Equate the RHS of Eq.~\ref{Eq1} and Eq.~\ref{Eq2}, 
    \eqn{ J_z J_- \ket{z} = z \hbar J_- \ket{z} - \hbar J_- \ket{z} = (z-1) \hbar J_- \ket{z} \label{loweringop} } 
    Eq.~\ref{loweringop} implies that $J_-$ keeps us in the same `family'/eigen-vector which is $\ket{z}$, though lower the eigenvalue by 1: $J_z$'s original eigenvalue is $z\hbar$; after applying $J_-$, $J_z$ has an eigenvalue of $(z-1) \hbar$. 
    
  \item Following the last bullet point, we must have, 
    \eqn{ J_- \ket{z} = \alpha \hbar \ket{z-1} }
    To find out the magnitude of $\alpha$, we evaluate
    \eqn{  \bra{z} J_+ J_- \ket{z} &= |\alpha|^2 \hbar^2  }
    Start by evaluating $J_+, J_-$ then substitute back into the above expression, 
    \begin{align}
      J_+ J_- &= (J_x + i J_y) (J_x - iJ_y) = J_x^2 + i (J_y J_x - J_x J_y) + J_y^2 \\
      &= J_x^2 + J_y^2 + \hbar J_z = J^2 - J_z^2 + \hbar J_z \\
      \bra{z} J^2 - J_z^2 + J_z \hbar \ket{z} &= |\alpha|^2 \hbar^2 \\
      \bra{z} J^2 \ket{z} - z^2 \hbar^2 + z^2 \hbar^2 &= |\alpha|^2 \hbar^2 \\
      \bra{z} J^2 \ket{z} &= |\alpha|^2 \hbar^2 
    \end{align}
    To help understanding, we define for some unknown $\beta$, 
    \eqn{ J^2 \ket{z} = \beta \hbar \ket{z} }
    Then the $\bra{z} J^2 \ket{z}$ term is kind of like the $\beta^2 \hbar^2$ term that keeps $J^2$ in the same family. 

  \item We cannot infinitely lower $z$. That is, the $\beta$ term has to satisfy the following three relations: 
    \begin{align}
      \left\{ \begin{array}{c} 
        z_{\max} - z_{\min} = \mathrm{integer}  \\
        \beta - z_{\min}^2 + z_{\min} = 0 \\
        \beta - z_{\max}^2 - z_{\max} = 0
      \end{array}
      \right. 
    \end{align}
    The only solution is, 
    \eqn{ z_{\min} = - z_{\max} = \left\{ \begin{array}{cc} \mathrm{integer} & \mathrm{Bosons} \\ \mbox{half integer} & \mathrm{Fermions}  \end{array} \right.   }

  \item If we define $j = z_{\max}$, and $m = z \in [-j, j]$, then we have 
    \eqn{ |\alpha| = \sqrt{j(j+1) - m(m-1)} }
    More specifically, 
    \eqn{ \Aboxed{J^2 \ket{j m} &= j(j+1) \hbar^2 \ket{j m}}  \label{J2-eq}}
    \eqn{ \Aboxed{J_z \ket{j m} &= m\hbar \ket{j m} }  }
    \eqn{ \Aboxed{ J_{\pm} \ket{j m} &= \sqrt{j(j+1) - m(m\pm 1)} \hbar \ket{jm\pm 1} } }
    Eq.~\ref{J2-eq} means there is quantum fluctuation in $J_x, J_y$. This is the reason people typically draw $\vec{J}$ on a sphere with radius $\sqrt{j(j+1) \hbar}$, and the direction is represented by the basis $\ket{jm}$. The circular motion comes from, if we make a $z$ measurement and get $m=j$, then we know the average $x$ measurement should be zero from 
        \eqn{ \bra{m=j} J_x \ket{m=j}  = 0} 
        But the fluctuation in $x,y$ are not zero, as we don't know exactly what they are, only the sum of their products: 
        \eqn{ \expect{J_x^2} + \expect{J_y^2} + (j \hbar)^2 = j^2 \hbar^2 + j^2 \hbar^2 }
  \end{enumerate}
\end{enumerate}


  \topic{Spin Angular Momentum}
 Consider a half-spin particle (neutrons, protons, electrons), that is $j = 1/2$. We can use the matrix notation, where bra becomes row vector, ket becomes column vector, and scalar becomes matrix. We can re-write the ket basis into 
    \eqn{ \ket{\frac{1}{2}} &= \left( \begin{array}{c} 1 \\ 0 \end{array} \right) & \ket{-\frac{1}{2}} &= \left( \begin{array}{c} 0 \\ 1 \end{array} \right) }
    Then we can solve the $\frac{\hbar}{2} \ket{\frac{1}{2}} = J_z \ket{\frac{1}{2}}, - \frac{\hbar}{2} \ket{-\frac{1}{2}} = J_z \ket{-\frac{1}{2}}$ equations for the-now-matrix-$J_z$: 
    \begin{align}
      \frac{\hbar}{2}  \left( \begin{array}{c} 1 \\ 0 \end{array} \right) &=  \left( \begin{array}{cc} a & c \\ b & d   \end{array} \right)  \left( \begin{array}{c} 1 \\ 0 \end{array} \right) = \begin{array}{c} a \\ b \end{array} \\
      - \frac{\hbar}{2}  \left( \begin{array}{c} 0 \\ 1 \end{array} \right) &=  \left( \begin{array}{cc} a & c \\ b & d   \end{array} \right)  \left( \begin{array}{c} 0 \\ 1 \end{array} \right) = \begin{array}{c} c \\ d \end{array} \\
      J_z &= \frac{\hbar}{2} \left( \begin{array}{cc} 1 & 0 \\ 0 & -1 \end{array} \right) 
    \end{align}
    Similarly we can solve for the matrix representation of $J_+, J_-$ as well, 
    \begin{align}
      J_+ \ket{ \frac{1}{2} } &= 0  \\
      \left( \begin{array}{c} a \\ b \end{array} \right) &= 0 \\
      J_+ \ket{ - \frac{1}{2} } &= \hbar \sqrt{-j(j+1) - m(m+1)} \ket{\frac{1}{2} }  \\
      &= \hbar \sqrt{ \frac{1}{2} \frac{3}{2} - \left( - \frac{1}{2} \right) \left( - \frac{1}{2} + 1 \right) } \ket{ \frac{1}{2} } \\
      &= \ket{ \frac{1}{2} } \\
      \Aboxed{J_+ &= \hbar \left( \begin{array}{cc} 0 & 1 \\ 0 & 0 \end{array} \right)}
    \end{align}
    We know that $J_-$ is just the transpose of $J_+$, hence, 
    \eqn{ \Aboxed{J_- &= \hbar \left( \begin{array}{cc} 0 & 0 \\ 1 & 0 \end{array} \right)}}
    Knowing what $J_+, J_-$ are, and knowning that $J_+ = J_x + i J_y, J_- = J_x - iJ_y$, and knowing that $J_i = \frac{\hbar}{2} \sigma_i$ where $\sigma_i$ is the Pauli matrix obeying $[ \sigma_i, \sigma_j] = 2 \epsilon_{ijk} \sigma_k$, we can write $J_x, J_y, J_z$: 
    \begin{align}
      J_x &= \frac{\hbar}{2} \left( \begin{array}{cc} 0 & 1 \\ 1 & 0 \end{array} \right) \\
      J_y &= \frac{\hbar}{2} \left( \begin{array}{cc} 0 & -i \\ i & 0 \end{array} \right) \\
      J_z &= \frac{\hbar}{2} \left( \begin{array}{cc} 1 & 0 \\ 0 & -1 \end{array} \right) 
    \end{align}


Background: the Levi-Civita symbols:
\begin{enumerate}
\item Index rule: summation is implied when different index shows up in adjacent terms:
  \eqn{ w_i = \epsilon_{ijk} n_j V_k = \Sum_j \Sum_k \epsilon_{ijk} n_j V_k }
\item Changing index: 
  \eqn{ \epsilon_{ijk} = - \epsilon_{jik} = -\epsilon_{ikj} }
  \eqn{ \epsilon_{ijk} \epsilon_{ij'k'} = \delta_{jj'} \delta_{kk'} - \delta_{jk'} \delta_{j'k} }
\item Final results: other terms are 0, 
\eqn{ \epsilon_{123} &= \epsilon_{231} = \epsilon_{312} = 1 & \epsilon_{213} &= \epsilon_{312} = \epsilon_{132} = -1 }
\end{enumerate}


%%%%%%%%%%%%%%%% %%%%%%%%%%%%%%%%%%%%%%%%%%%%%%%%%%%
\topic{Orbital Angular Momentum}
This is similar to its classical description of angular momentum. 

\subtopic{Construct Cartesian Components of $\hat{L}$}
We define the orbital angular momentum like:
\begin{align}
\hat{\uline{L}} &= \hat{\uline{r}} \cross \hat{\uline{p}} \\
\hat{\uline{L}}_x &= \hat{y} \hat{p}_z - \hat{z} \hat{p}_y = - i\hbar \left( y \ppz - z \ppy \right) \\
\hat{\uline{L}}_y &= \hat{z} \hat{p}_x - \hat{z} \hat{p}_x = - i\hbar \left( z \ppx - x \ppz \right) \\
\hat{\uline{L}}_z &= \hat{x} \hat{p}_y - \hat{y} \hat{p}_x = - i\hbar \left( x \ppy - y \ppx \right) 
\end{align}

\subtopic{Check the Components We Just Constructed}
The question we want to ask is, `can we find the eigenvalues of each of the operators simultaneously?'

To answer the above question, we consider whether the components commute with each other. Because if $\left[ \hat{L}_x, \hat{L}_y \right] = 0$, that is to say we can pin $L_x, L_y$ at the same time. 

Though when we derive it for real (see notes), they come out to be:
\eqn{ \left[ \hat{L}_x, \hat{L}_y \right] = i \hbar ( \hat{x} \hat{P}_y - \hat{y} \hat{P}_x) = i\hbar \hat{L}_z }
\eqn{ \left[ \hat{L}_y, \hat{L}_z \right] = i \hbar ( \hat{y} \hat{P}_z - \hat{z} \hat{P}_y) = i\hbar \hat{L}_x }
\eqn{ \left[ \hat{L}_z, \hat{L}_x \right] = i \hbar ( \hat{z} \hat{P}_x - \hat{x} \hat{P}_z) = i\hbar \hat{L}_y }

That is to say, $\hat{L}_x, \hat{L}_y, \hat{L}_z$ do not have common eigenstates, and that we cannot find $L_x, L_y, L_z$ simultaneously. 

\subtopic{Define the Orbital Angular Momentum Operator $\Lhat^2$}
What the above argument leads to is the $\hat{L}^2$,  a more physical term, and the square root of its eigenvalue is the angular momentum. 
\eqn{ \left[ \hat{L}^2, \hat{L}_x   \right] =  \left[ \hat{L}^2, \hat{L}_y   \right] =  \left[ \hat{L}^2, \hat{L}_z   \right] = 0   }
We can solve for the total angular momentum and the azimuthal component simultaneously in a coordinate system as illustrated in Figure~\ref{3DCS}. 
\begin{figure}
    \centering
    \includegraphics[width=2in]{images/qm/3DCS.png}
    \caption{Set-up of the 3D Coordinate System\label{3DCS}}
\end{figure}
\eqn{ \hat{L}_z = - i \hbar \ppphi }
\eqn{ \hat{L}^2 =  - \hbar^2 \left[ \frac{1}{\sin \theta} \pptheta \left( \sin \theta \pptheta \right) + \frac{1}{\sin^2 \theta} \ppphin2  \right] }

\subtopic{Define the Total Angular Momentum $\Jhat$}
We define the Total Angular Momentum as:
\eqn{ \Jhat = \Lhat + \Shat }
Notice we cannot solve for the three components of $\Jhat$ simultaneously neither, because: 
\eqn{ \left[ \Jhat_x, \Jhat_y \right] = i \hbar \Jhat_z,  \left[ \Jhat_y, \Jhat_z \right] = i \hbar \Jhat_x, \left[ \Jhat_z, \Jhat_x \right] = i \hbar \Jhat_y }


\subtopic{Eigenvalues of $\Lhat, \Jhat$}
See Liboff 9.3 for how we get the following equations: 
\eqn{ \boxed{ \hat{L}^2 \phi_{l,m} (\theta, \phi) = \hbar^2 l (l+1) \phi_{l,m} (\theta, \phi ), \fsp \fsp \hat{L}_z \phi_{l,m} (\theta, \phi) = \hbar m \phi_{l,m} (\theta, \phi ) } }
in which $l = 0,1,2, \cdots, m = -l, -l+1, \cdots, 0, \cdots l$. If we solve for $\hat{L}_x$ or $\hat{L}_y$ instead we will reach the same results as above. 

Similarly $\Jhat$ would give us:
\eqn{  \Jhat^2 \phi_{l,m} (\theta, \phi) = \hbar^2 j (j+1) \phi_{l,m} (\theta, \phi ), \fsp \fsp \Jhat_z \phi_{l,m} (\theta, \phi) = \hbar m_j \phi_{l,m} (\theta, \phi )  }
in which $j = 0,1/2,1,3/2,2, \cdots, m = -j, \cdots, j$. If we solve for $\Jhat_x$ or $\Jhat_y$ instead we will reach the same results as above. 

\subtopic{Eigenfunctions $\phi_{l,m}$ is Spherical Harmonics $Y_l^m(\theta, \phi)$}
The eigenfunction in the above equation, $\phi_{l,m}$, are commonly called the \textbf{Spherical Harmonics $Y_l^m (\theta, \phi)$}:
\eqn{ Y_l^m (\theta, \phi) = \frac{1}{\sqrt{2 \pi}} e^{im\phi} P_l^m (\phi)   }
A couple of things about the Spherical Harmonics:
\begin{itemize}
\item $\psi( r, \theta, \phi) = R(r) Y_{lm} (\theta, \phi)$. 
\item $\int_0^{2\pi} \dphi \int_0^{\pi} \sin \theta \dtheta |Y_{lm} (\theta, \phi) |^2 = 1.$
\item Spherical Harmonics also implies that the unit of angular momentum is $\hbar$.
\item Degeneracy: \textbf{For a given $l$ value, there are $2l+1$ number of degeneracy.} For instance, for $l=5$, we have 11 eigenstates $Y_5^5, Y_5^4, \cdots Y_5^{-5}$ that correspond to the same $l$, or the same $L^2 = 30 \hbar^2$. That is, for the same $L^2$, the projection onto the azimuthal plan are degenerate.  
\item $L_z$ is not continuous. Given a $L^2$, we can draw a bunch of cones, each surface describe the superposition of possible eigenfunctions. L will never entirely align with the z axis. 
\end{itemize}


\subtopic{Summary of Quantum Numbers}
\begin{enumerate}
\item Orbital Angular Momentum Quantum Number $l$: integers, $0 \le l \le n$. A subset of j is the solution from orbital component. 
\item Total Angular Momentum Quantum Number $j$: integer steps, $|l-s|, \cdots, |l+s|$. It completely construct $l$ and $s$. 
\item $m_j$: $-j, \cdots j$ (includes 0 when j is an integer, and does not include 0 when j is a half-integer). It's degeneracy is $2j+1$. 
\end{enumerate}

\begin{table}[h!]
\begin{tabular}{|p{1.5in}|p{1.5in}|p{1.5in}|p{1.5in}|} \hline
 & $\Lhat$ & $\Shat$ &$\Jhat = \Lhat + \Shat$ \\ \hline
\multirow{3}{*}{Commutating Relations} &
   $\left[ \Lhat_x, \Lhat_y \right] = i \hbar \Lhat_z$ &  $\left[ \Shat_x, \Shat_y \right] = i \hbar \Shat_z$ &  $\left[ \Jhat_x, \Jhat_y \right] = i \hbar \Jhat_z$ \\
&  $\left[ \Lhat_y, \Lhat_z \right] = i \hbar \Lhat_x$ &  $\left[ \Shat_y, \Shat_z \right] = i \hbar \Shat_x$ &  $\left[ \Jhat_y, \Jhat_z \right] = i \hbar \Jhat_x$ \\
&  $\left[ \Lhat_z, \Lhat_x \right] = i \hbar \Lhat_y$ &  $\left[ \Shat_z, \Shat_x \right] = i \hbar \Shat_y$ &  $\left[ \Jhat_z, \Jhat_x \right] = i \hbar \Jhat_y$ \\ \hline
Quantum Numbers & $ l = 0,1,2,\cdots $ & $s = 0, 1/2, 1, \cdots$               & $ j =|l-s|,\cdots, |l+s|$ \\
(all in integer steps) & $-l \le m_l \le l  $  & $ -s \le m_s \le s$  & $-j \le m_j \le j$  \\ \hline
\multirow{2}{*}{Eigenvalues} 
& $\expect{L^2} = \hbar^2 l (l+1)$ 
& $\expect{S^2} = \hbar^2 s (s+1)$
& $\expect{J^2} = \hbar^2 j(j+1)$\\ 
& $\expect{L_z} = \hbar m_l$ 
& $\expect{S_z} = \hbar m_s$ 
& $\expect{J_z} =  \hbar m_j$  \\ \hline
\end{tabular}
\caption{Comparison of Quantum Numbers $l,s,j$}
\label{quantum-numbers}
\end{table}


\topic{Additions of Angular Momentum}
Examples:
\begin{enumerate}
\item $2e^-: \Lhat = \Lhat_1 + \Lhat_2 $ 
\item $ 1 e^-: \Jhat = \Lhat + \Shat$
\item \ce{^2H} = p+n: l =0. $\Jhat = \Shat_p + \Shat_n$. 
\end{enumerate}

\uline{Example 1: Adding Two Orbital Momentum:} we want to find the $(l,m)$ associated with $\Lhat= \Lhat_1 + \Lhat_2$ from the four quantum numbers $l_1, m_1, l_2, m_2$. 
\begin{itemize}
\item $\Lhat^2 = (\Lhat_1 + \Lhat_2)^2 $
\item $ \Lhat_z = \Lhat_{1z} + \Lhat_{2z} \Rightarrow m_{\mathrm{max}} = m_{\mathrm{1,max}} + m_{\mathrm{2,max}} = l_1 + l_2.$
$\fsp l_{\mathrm{max}} = m_{\mathrm{max}} = l_1 + l_2.$
\item $ \mbox{Total \# of independent states } N = (2 l_1 + 1) (2l_2 + 1) = \Sum_{l_{\mathrm{min}}}^{l_{\mathrm{max}}} (2l+1).$
$\fsp\Rightarrow l_{\mathrm{min}} = |l_2 - l_1 |.$ That is,
\eqn{ l = |l_2 - l_1|, \cdots , l_1 + l_2}
\end{itemize}

\uline{Example 2: Adding Two Electrons}

Given: $ 2e^-$, 1 $e^-$ \@ $l_1 = 1$, 1 $e^-$ \@ $l_2 = 2$. Answer: 
\begin{itemize}
\item $l = 1,2,3$.
\item $L = \hbar \sqrt{l (l+1)} = \hbar \sqrt{2}, \hbar \sqrt{6}, \hbar \sqrt{12}.$.
\item $N = \Sum_1^3 (2l+1) = 3 + 5 + 7 = 15$, or $N = 3 \times 5 = 15$. 
\end{itemize}





\end{document}
